\documentclass{MathNotes}

\newenvironment{example}[1]{\begin{BlueBox}{Example}{#1}}{\end{BlueBox}}
\newenvironment{definition}[1]{\begin{RedBox}{Definition}{#1}}{\end{RedBox}}
\newenvironment{note}[1]{\begin{YellowBox}{Note}{#1}}{\end{YellowBox}}
\newenvironment{theorem}[1]{\begin{GrayBox}{Theorem}{#1}}{\end{GrayBox}}
\newenvironment{practice}[1]{\begin{PurpleBox}{Practice}{#1}}{\end{PurpleBox}}
\newenvironment{graph}{\begin{tikzpicture}[node distance={0.65in}, thick, auto=center,every node/.style={draw,circle,fill=green!10}]}{\end{tikzpicture}}

\newcommand{\br}{
	\begin{center}
		\line(1,0){4ex}
	\end{center}
}
\newcommand{\bl}{
	\newline$ $\newline
}
\newcommand{\continued}{
	\mbox{}
	\vfill
	\textbf{Continued on Next Page\ldots}\newpage
}
%----------------------Author Information-----------------
\title{Speed Running Discrete Mathematics}
\author{Minh Nguyen}

%---------------------Document Begin-----------------------
% \usepackage{layout}
\begin{document}
% \begin{center}
%     \layout*
% \end{center}
\newpage
\maketitle
\pagenumbering{gobble}
\vfill
\tableofcontents
\newpage
\section*{Author's Notes}
This actually isn't the first copy of my discrete math notes\ldots I had an earlier copy that got corrupted, so now I'm just going to constantly upload to GitHub because I'm afraid of them getting wiped again \emoji{sob}
\br{}

These notes are based off of the textbook \textit{Discrete Mathematics and Its Applications} by \textit{Kenneth H. Rosen}, as well as from the lectures of \textit{Serdar Erbatur} from the \textit{Fall 2023} semester.
\br{}
If you have any complaints, or suggestions regarding these notes, please
email me at \newline\href{mailto:minh.nguyen7@utdallas.edu}{mdn220004@utdallas.edu}
\newpage
\pagenumbering{arabic}

\section{Propositional Logic}\label{sec:propositional-logic}
\begin{definition}{Proposition}
	Declarative statements that are either \texttt{true} or \texttt{false}
\end{definition}

\begin{table}[h!]\label{tab:prop-examples}
	\centering
	\caption{Examples of propositions}
	\begin{tabular}{lc}
		\multicolumn{1}{c}{\textbf{Statement}} & \multicolumn{1}{c}{\textbf{Proposition?}} \\
		\midrule
		$1+1=2$                                & \emoji{check-mark}                        \\
		What class are ya takin?               & \emoji{no-entry}                          \\
		I am happy                             & \emoji{check-mark}
	\end{tabular}
\end{table}

Propositions can be combined to form another proposition with the use of \textit{logical operators}
\begin{note}{}
	Common labels for propositions in discrete mathematics include letters like $P,Q,R,S$\ldots
\end{note}

\begin{table}[h!]\label{tab:logical-operators}
	\centering
	\caption{Logical Operators in Discrete Mathematics}
	\begin{tabular}{clc}
		\multicolumn{1}{c}{\textbf{Symbol}}   &
		\multicolumn{1}{c}{\textbf{Meaning} } &
		\multicolumn{1}{c}{\textbf{Expression}}                                            \\
		\midrule
		$\lnot$                               & negation / not             & $\lnot P$     \\
		$\land$                               & conjunction / and          & $P\land Q$    \\
		$\lor$                                & disjunction / or           & $P\lor Q$     \\
		$\oplus$                              & exclusive disjunction/ xor & $P\oplus Q$   \\
		$\implies$                            & implication / conditional  & $P\implies Q$ \\
		$\iff$                                & biconditional              & $P\iff Q$     \\
	\end{tabular}
\end{table}

\begin{note}{Logical Operator Precedence}\label{order-of-operations}
	Order matters when it comes to evaluating logical operators:
	\begin{enumerate}
		\item negation
		\item conjunction
		\item disjunctions
		\item conditionals
	\end{enumerate}
	Where negation is evaluated first, and conditionals last.
\end{note}

\newpage
\begin{multicols}{2}
	\begin{theorem}{More on Conditionals}\label{th:conditionals-extra}
		Conditionals can also be expressed in three other ways:
		\bl
		\textbf{Contrapositive:} $\lnot Q\implies\lnot P$
		\bl
		\textbf{Converse:} $Q\implies P$
		\bl
		\textbf{Inverse:} $\lnot P\implies\lnot Q$
	\end{theorem}
	\begin{example}{}
		\textbf{Conditional:} If \underline{it is raining}, then \underline{I am not going to town}
		\bl
		\textbf{Contrapositive:} If \underline{I go to town}, then \underline{it is not raining}
		\bl
		\textbf{Converse:} If \underline{I do not go to town}, then \underline{it is raining}
		\bl
		\textbf{Inverse:} If \underline{it is not raining}, then \underline{I am going to town}
	\end{example}
\end{multicols}

\begin{definition}{Truth Table}
	They are used as a way of seeing all possible values of a proposition
\end{definition}

\begin{table}[h!]\label{tab:truth-table-example}
	\centering
	\caption{Truth Table of $P\implies Q$}
	\begin{tabular}{cc|c}
		$P$ & $Q$ & $P\implies Q$ \\
		\hline
		F   & F   & T             \\
		F   & T   & T             \\
		T   & F   & F             \\
		T   & T   & T             \\
	\end{tabular}
\end{table}

\subsection{Propositional Equivalencies}\label{sec:prop-equivalencies}
\begin{definition}{Equivalencies}\label{def:equivalencies}
	A proposition is a\ldots
	\begin{itemize}
		\item \textbf{Tautology} if it is \texttt{true} in \textit{every case}
		\item \textbf{Contradiction / Fallacy} if it is \texttt{false} in \textit{every case}
		\item \textbf{Contingency} if \textit{neither} is the case
	\end{itemize}
\end{definition}

\begin{table}[h!]\label{tab:tautology-contradiciton-ex}
	\centering
	\caption{Example of Tautology and Contradiction}
	\begin{tabular}{c|c|c|c}
		$P$ & $\lnot P$ & $P\lor\lnot P$ & $P\land\lnot P$ \\
		\hline
		T   & F         & T              & F               \\
		F   & T         & T              & F
	\end{tabular}
\end{table}

\begin{definition}{Logical Equivalency ($\equiv$)}\label{th:logical-equiv}
	Compound propositions $P$ and $Q$ are \textit{logically equivalent} if $P\iff Q$ is a \textit{tautology}. This is expressed as \[P\equiv Q\]
\end{definition}

Below is a table of useful logical equivalencies

\begin{table}[h!]
	\centering
	\caption{Logical Equivalencies}
	\begin{tabular}{ll}
		\textbf{Name}                 & \textbf{Equivalence}                            \\
		\midrule
		\multirow{2}{*}{Identity}     & $P\land\text{T} \equiv P$                       \\
		                              & $P\lor\text{F} \equiv P$                        \\
		\hdashline{}
		\multirow{2}{*}{Idempotent}   & $P\land P \equiv P$                             \\
		                              & $P\lor P \equiv P$                              \\
		\hdashline{}
		\multirow{2}{*}{Domination}   & $P\lor\text{T} \equiv \text{T}$                 \\
		                              & $P\land\text{F} \equiv \text{F}$                \\
		\hdashline{}
		\multirow{2}{*}{Negation}     & $P\lor\lnot P \equiv \text{T}$                  \\
		                              & $P\land\lnot P \equiv \text{F}$                 \\
		\hdashline{}
		Double Negation               & $\lnot(\lnot P)\equiv P$                        \\
		\hdashline{}
		\multirow{2}{*}{Commutative}  & $P\land Q\equiv Q\land P$                       \\
		                              & $P\lor Q\equiv Q\lor P$                         \\
		\hdashline{}
		\multirow{2}{*}{Associative}  & $(P\land Q)\land R\equiv P\land(Q\land R)$      \\
		                              & $(P\lor Q)\lor R\equiv P\lor(Q\lor R)$          \\
		\hdashline{}
		\multirow{2}{*}{Distributive} & $P\land(Q\lor R)\equiv(P\land Q)\lor(P\land R)$ \\
		                              & $P\lor(Q\land R)\equiv(P\lor Q)\land(P\lor R)$  \\
		\hdashline{}
		\multirow{2}{*}{De Morgan's}  & $\lnot(P\land Q)\equiv\lnot P\lor\lnot Q$       \\
		                              & $\lnot(P\lor Q)\equiv\lnot P\land\lnot Q$       \\
		\hdashline{}
		\multirow{2}{*}{Absorption}   & $P\land(P\lor Q)\equiv P$                       \\
		                              & $P\lor(P\land Q)\equiv P$                       \\
	\end{tabular}
\end{table}

The use of showing the equivalencies between two compound propositions is called a
\textit{conditional-disjunction equivalence}
\begin{example}{Conditional-Disjunction Equivalence}\label{ex:conditional-disjunction-equivalence}
	\[P\implies Q\equiv\lnot P\lor Q\]
\end{example}

This can be proven with the use of a truth table \emoji{smiling-face-with-hearts}
\continued

\begin{table}[h!]\label{tab:conditional-disjunction-equivalence}
	\centering
	\caption{Conditional-Disjunction Equivalence Proof}
	\begin{tabular}{cc|c|c|c}
		$P$ & $Q$ & $\lnot P$ & $\lnot P\lor Q$ & $P\implies Q$ \\
		\midrule
		F   & F   & T         & T               & T             \\
		F   & T   & T         & T               & T             \\
		T   & F   & F         & F               & F             \\
		T   & T   & F         & T               & T             \\
	\end{tabular}
\end{table}

\subsection{Predicates and Quantifiers}\label{sec:predicates-quantifiers}

\begin{note}{}
	So far, propositional logic can only handle \textit{singular} subjects. It can't handle statements such as:
	\begin{itemize}
		\item All computer science students can program well
		\item $3x+4\geq0$
	\end{itemize}
\end{note}

\begin{multicols}{2}
	\begin{definition}{Predicate Logic}\label{def:pred-logic}
		When you have a proposition that contains a variable. It is typically written as a \textit{propositional function}, $P(x)$, where $x$ is the subject for the predicate $P$
	\end{definition}

	\begin{example}{}\label{ex:pred-logic}
		\begin{itemize}
			\item $F(x)=\text{``}x>3\text{''}$
			\item $P(x)=\text{``}x\text{ looks beautiful!''}$
		\end{itemize}
	\end{example}
\end{multicols}

\begin{note}{Multi-variable Propositional Functions}\label{note:prop-func-multi}
	Propositional functions may also contain more than just one argument:
	\[P(x,y)\]
\end{note}

\begin{definition}{Quantifiers}\label{def:quantifiers}
	They define the range of which a proposition holds \texttt{true}, and can be nested to produce \textit{nested quantifiers}
\end{definition}

\marginnote{$\forall x.P(x)$ may also be written as $\forall xP(x)$, and the same holds for the other quantifiers}
\begin{table}[h!]\label{tab:quantifiers}
	\centering
	\caption{Quantifiers in Discrete Mathematics}
	\begin{tabular}{l l l}
		\multicolumn{1}{c}{\textbf{Quantifier}} &
		\multicolumn{1}{c}{\textbf{Expression}} &
		\multicolumn{1}{c}{\textbf{In English}}                                                                                         \\
		\midrule
		Universal Quantifier                    & $\forall x. P(x)$  & $P(x)$ is \texttt{true} for every $x$ in its domain              \\
		\hdashline{}
		\multirow{3}{*}{Existential Quantifier} & $\exists x. P(x)$  & There exists $x$ where $P(x)$ is \texttt{true}                   \\
		                                        & $\nexists x. P(x)$ & There does not exist $x$ where $P(x)$ is \texttt{true}           \\
		                                        & $\exists! x. P(x)$ & There exists \textit{only one} $x$ where $P(x)$ is \texttt{true}
	\end{tabular}
\end{table}

\begin{example}{Nested Quantifiers}\label{ex:nested-quantifiers}
	\centering
	\[\forall x\exists y.(x+y=0)\] Translates to: ``For \textit{every} $x$ \textit{there exists} a $y$ such that $x+y=0$''
\end{example}
\subsection{Inference Rules and Proofs}
\begin{multicols}{2}
	\begin{definition}{Argument}\label{def:argument}
		A sequence of statements that have a conclusion
	\end{definition}

	\begin{definition}{Valid}\label{def:valid}
		The conclusion, the final statement of the argument, must follow from its premises
		\newline
		(i.e. premises $\implies$ conclusion)
	\end{definition}

	\begin{definition}{Premise}\label{def:premise}
		The preceding statements of a mathematical argument that lead to a conclusion
	\end{definition}

	\begin{definition}{Fallacy}
		Incorrect reasoning in discrete mathematics that leads to an invalid argument
	\end{definition}
\end{multicols}


\begin{example}{Argumentative Form}\label{ex:argumentative-form}
	Arguments may be written as this: $\big((P\implies Q)\land P\big)\implies Q$, or in argumentative form:
	\begin{align*}
		           & P\implies Q                 \\
		           & \underline{P\hspace{3.5em}} \\
		\therefore & Q
	\end{align*}
\end{example}

The next page contains a table of inference rules
\newpage
\begin{table}[h!]\label{tab:inference-rules}
	\centering
	\caption{Rules of Inference}
	\begin{tabular}{lll}
		\multicolumn{1}{c}{\textbf{Rule}}                          &
		\multicolumn{1}{c}{\textbf{Expression}}                    &
		\multicolumn{1}{c}{\textbf{Tautology}}                            \\
		\midrule
		Modus ponens                                               &
		$\begin{array}{rl}
				            & P                       \\
				            & \underline{P\implies Q} \\
				 \therefore & Q\end{array}$                    &
		$\big(P\land(P\implies Q)\big)\implies Q$                         \\
		\hdashline{}
		Modus tollens                                              &
		$\begin{array}{rl}
				            & \lnot Q                 \\
				            & \underline{P\implies Q} \\
				 \therefore & \lnot P\end{array}$                    &
		$\big(\lnot Q\land(P\implies Q)\big)\implies \lnot P$             \\
		\hdashline{}
		Hypothetical syllogism                                     &
		$\begin{array}{rl}
				            & P\implies Q             \\
				            & \underline{Q\implies R} \\
				 \therefore & P\implies R\end{array}$                    &
		$\big((P\implies Q)\land(Q\implies R)\big)\implies (P\implies R)$ \\
		\hdashline{}
		Disjunctive syllogism                                      &
		$\begin{array}{rl}
				            & P\lor Q                            \\
				            & \underline{\lnot P\hspace{1.25em}} \\
				 \therefore & Q\end{array}$ &
		$\big((P\lor Q)\land\lnot P\big)\implies Q$                       \\
		\hdashline{}
		Addition                                                   &
		$\begin{array}{rl}
				            & \underline{P\hspace{2em}} \\
				 \therefore & P\lor Q\end{array}$       &
		$P\implies(P\lor Q)$                                              \\
		\hdashline{}
		Simplification                                             &
		$\begin{array}{rl}
				            & \underline{P\land Q} \\
				 \therefore & P\end{array}$                       &
		$(P\land Q)\implies P$                                            \\
		\hdashline{}
		Conjunction                                                &
		$\begin{array}{rl}
				            & P                            \\
				            & \underline{Q\hspace{1.25em}} \\
				 \therefore & P\land Q\end{array}$       &
		$\big((P)\land(Q)\big)\implies P\land Q$                          \\
		\hdashline{}
		Resolution                                                 &
		$\begin{array}{rl}
				            & P\lor Q                   \\
				            & \underline{\lnot P\lor R} \\
				 \therefore & Q\lor R\end{array}$                  &
		$\big((P\lor Q)\land(\lnot P\lor R)\big)\implies (Q\lor R)$       \\
		\hdashline{}
	\end{tabular}
\end{table}

\begin{table}[h!]\label{tab:inference-rules-quantified}
	\centering
	\caption{Rules of Inference for Quantified Statements}
	\begin{tabular}{ll}
		\multicolumn{1}{c}{\textbf{Rule}} &
		\multicolumn{1}{c}{\textbf{Expression}}                         \\
		\midrule
		Universal Instantiation           &
		$\begin{array}{rl}
				            & \underline{\forall x.P(x)} \\
				 \therefore & P(c)\end{array}$                        \\
		\hdashline{}
		Universal Generalization          &
		$\begin{array}{rl}
				            & \underline{P(c) \text{ for an arbitrary } c} \\
				 \therefore & \forall x.P(x)\end{array}$        \\
		\hdashline{}
		Existential Instantiation         &
		$\begin{array}{rl}
				            & \underline{\exists x.P(x)\hspace{7em}} \\
				 \therefore & P(c)\text{ for some element } c\end{array}$ \\
		\hdashline{}
		Existential Generalization        &
		$\begin{array}{rl}
				            & \underline{P(c) \text{ for an arbitrary } c} \\
				 \therefore & \forall x.P(x)\end{array}$        \\
	\end{tabular}
\end{table}

\begin{definition}{Proof}\label{def:proof}
	\underline{Valid arguments} that establish the \texttt{truth} of mathematical statements
\end{definition}

\begin{definition}{Theorem}\label{def:theorem}
	A statement or claim that can be proven using:
	\begin{itemize}
		\item definitions
		\item other theorems
		\item axioms
		\item inference rules
	\end{itemize}
	They are also referred to as ``Lemma'', ``Proposition'', or ``Corollary''
\end{definition}
There are many different ways of proving a theorem. Let's assume a conditional statement $P\implies Q$\ldots
\begin{multicols}{2}
	\begin{definition}{Direct Proof}\label{def:direct-proof}
		When the first step is the assumption that $P$ is
		\texttt{true} and the following steps that lead up to $Q$ is also \texttt{true}
	\end{definition}

	\begin{definition}{Indirect Proof}\label{def:indirect-proof}
		Proofs that do not start with the premises and end with conclusion (the opposite of a direct proof). Ways of doing direct proofs involve \textit{proof by contraposition}, \textit{proof by contradiction}, and much more\ldots
	\end{definition}

	\begin{example}{Proof by Contraposition}\label{ex:contraposition-proof}
		$P\implies Q$ can be proved \texttt{true} if $\lnot Q\implies P$, its contraposition, can also be proved. This is because a contraposition and a conditional proposition are tautologies
	\end{example}

	\begin{example}{Proof by Contradiciton}\label{ex:contradiciton-proof}
		To prove $P$, you must assume $\lnot P$ and derive that $\lnot P$ is \texttt{false}. If $\lnot P$ is \texttt{false}, then that must mean that $\lnot\lnot P$, or $P$, must be \texttt{true}
	\end{example}
\end{multicols}

% TODO: write about proof by equivalence, existence, and exhaustion
\newpage
\section{Set Theory}
\begin{multicols}{2}
	\begin{definition}{set}\label{def:set}
		A collection of \textit{unique} objects or elements
		\begin{itemize}
			\item $a\in A$ to state that $a$ is \textit{contained} in the set $A$
			\item $a\not\in A$ to indicate that $a$ \textit{is not} contained in $A$
		\end{itemize}
	\end{definition}

	\begin{note}{Defining Sets}\label{note:defining-sets}
		Roster method
		\begin{align*}
			A & = \{a,b,c,d\}                            \\
			B & = \{4,b,c,a\}                            \\
			C & = \bigl\{1, 2, \{3.0, 3.5\}, 4, 5\bigr\} \\
			D & = \{1, 2, C\}
		\end{align*}
		Set Builder Notation
		\begin{align*}
			E & = \{x\in\mathbb{N} \big| x=2k\text{ for some }k\in\mathbb{N}\} \\
			F & = \{\alpha \big| P(\alpha) \text{ is }\texttt{true}\}
		\end{align*}
	\end{note}
\end{multicols}

\begin{table}[h!]\label{tab:important-sets}
	\centering
	\caption{Important Sets}
	\begin{tabular}{lll}
		\multicolumn{1}{c}{\textbf{Set}}                           &
		\multicolumn{1}{c}{\textbf{Expansion}}                     &
		\multicolumn{1}{c}{\textbf{Description}}                         \\
		\midrule
		$\mathbb{N}$                                               &
		$\{0, 1, 2, 3,\cdots\}$                                    &
		Natural numbers                                                  \\
		$\mathbb{Z}$                                               &
		$\{\cdots,-1,0, 1,\cdots\}$                                &
		Integers                                                         \\
		$\mathbb{Z}^+$                                             &
		$\{1, 2, 3,\cdots\}$                                       &
		Positive integers                                                \\
		$\mathbb{Q}$                                               &
		$\{\frac{P}{Q}\big|P\in\mathbb{Z},Q\in\mathbb{Z},Q\neq0\}$ &
		Rational numbers                                                 \\
		$\mathbb{R}$                                               &   &
		Real numbers                                                     \\
		$\mathbb{R}^+$                                             &
		$\{x\big|x>0\}$                                            &
		Positive real numbers                                            \\
		$\mathbb{C}$                                               &   &
		Complex numbers                                                  \\
		$\varnothing$                                              &   &
		Empty set                                                        \\
	\end{tabular}
\end{table}

\newpage
\subsection{Subsets}
\begin{multicols}{2}
	\begin{theorem}{Set Equality}\label{th:set-equality}
		Given two sets $A$ and $B$:\[A\equiv B\iff\forall x.(x\in A\iff x\in B)\] is \texttt{true}
	\end{theorem}

	\begin{definition}{Subset ($\subseteq$)}
		$A$ is a subset of $B$ if \textit{all elements of} $A$ are also contained in $B$:
		\[A\subseteq B\iff\forall x.(x\in A\implies x\in B)\]
	\end{definition}
\end{multicols}

\begin{example}{Subsets}\label{ex:subsets}
	Let $A=\{2,3\},B=\{a,b,c,2,3\}$\newline
	\begin{multicols}{2}
		\begin{itemize}
			\item $A\subseteq B$  \texttt{true}\\
			\item $A\subseteq A$  \texttt{true}\\
			\item $\varnothing\subseteq A$  \texttt{true}\\
			\item $B\subseteq A$  \texttt{false}\\
		\end{itemize}
	\end{multicols}
\end{example}

\marginnote{This notation is seen in Section~\ref{def:cardinality}}
\begin{multicols}{2}
	\begin{definition}{Power Set}\label{def:power-set}
		The set of all subsets of the set\[\bigl|A\bigr|=n,\bigl|P(A)\bigr|=2^n\]
	\end{definition}

	\begin{example}{}\label{ex:power-set}
		Let $S=\{1,2\}$:\[P(S)=\bigl\{\varnothing,\{1\},\{2\},\{1,2\}\bigr\}\]
	\end{example}
\end{multicols}

\begin{definition}{Proper Subset ($\subset$)}
	It's a subset where $A\neq B$: \[A\subset B\iff\forall x.(x\in A\implies x\in B)\land A\neq B\]
\end{definition}

\subsection{Cardinality}\label{sec:cardinality}

\begin{multicols}{2}
	\begin{definition}{Cardinality}\label{def:cardinality}
		It's the number of unique elements in a set. It's denoted by $\bigl|A\bigr|$
	\end{definition}
	\begin{example}{}\label{ex:cardinality}
		\begin{tabular}{ll}
			$\big\{\{1, 2\}, 3\big\}$ & 2 elements \\
			$\{1,2,3\}=\{1,2,3,3\}$   & 3 elements \\
			$\{\varnothing\}$         & 1 element  \\
			$\{\}$                    & 0 elements \\
			$\{\varnothing\}$         & 1 element
		\end{tabular}
	\end{example}
	\begin{definition}{Intervals}\label{def:intervals}
		Sets of numbers \textit{between} two numbers $a$ and $b$ if
		$a,b\in\mathbb{R}\land a\leq b$
		\begin{itemize}
			\item $[a, b]=x\big|a\leq x\leq b$
			\item $[a, b)=x\big|a\leq x < b$
			\item $(a, b]=x\big|a < x\leq b$
			\item $(a, b)=x\big|a < x < b$
		\end{itemize}
	\end{definition}
\end{multicols}

\newpage
\begin{multicols}{2}
	\begin{definition}{Ordered Tuples}\label{def:ordered-tuples}
		\[(a_0,a_1,a_2,\cdots,a_n)\]
		An \textit{ordered collection} of unique elements
		\[(a,b,c)\neq(b,c,a)\]
	\end{definition}
	\begin{theorem}{Cartesian Products}\label{th:cartesian-products}
		Let $A$ and $B$ be sets:\[A\times B=\{(a,b)\big|a\in A,b\in B\}\]
	\end{theorem}
\end{multicols}
\begin{example}{Cartesian Product}
	Let $A=\{1,2\},B=\{a,b,c\}$:
	\[A\times B=\{(1,a),(1,b),(1,c),(2,a),(2,b),(2,c)\}\]
\end{example}

\subsection{Set Operations}
Let $A=\{1,2,3\},B=\{2,3,4,5\}$:
\begin{table}[h!]
	\centering
	\caption{Set Operations}
	\begin{tabular}{ccl}
		\multicolumn{1}{c}{\textbf{Expression}} &
		\multicolumn{1}{c}{\textbf{Meaning}}    &
		\multicolumn{1}{c}{\textbf{Result}}                                               \\
		\midrule
		$A\cup B$                               & $A$ union $B$        & $\{1,2,3,4,5\}$  \\
		$A\cap B$                               & $A$ intersection $B$ & $\{2,3\}$        \\
		$\bar{A}$                               & $A$ complement $B$   & $\{x\not\in A\}$ \\
	\end{tabular}
\end{table}
\begin{definition}{Membership Table}\label{def:membership-table}
	It's very similar to a truth table, where \texttt{true} means that an element exists within the set, and \texttt{false} means that the element isn't.
\end{definition}

\begin{table}[h!]
	\centering
	\caption{Membership Table Example}
	\begin{tabular}{cc|c|c}
		$A$            & $B$            & $A\cup B$      & $A\cap B$      \\
		\midrule
		\texttt{false} & \texttt{false} & \texttt{false} & \texttt{false} \\
		\texttt{false} & \texttt{true}  & \texttt{true}  & \texttt{false} \\
		\texttt{true}  & \texttt{false} & \texttt{true}  & \texttt{false} \\
		\texttt{true}  & \texttt{true}  & \texttt{true}  & \texttt{true}
	\end{tabular}
\end{table}

\newpage
\subsection{Functions}

\begin{multicols}{2}
	\begin{definition}{Function}\label{def:function}
		Function $f$ is denoted from set $A$ to set $B$:
		\[f:A\to B\]
		representing a relation that assigns each element of $A$ to \textit{exactly one} element
		of $B$
	\end{definition}

	\begin{example}{}\label{ex:functions}
		Let $A=\{1,2\},B=\{a,b\}$\[A\times B=\{(1,a),(1,b),(2,a),(2,b)\}\]
		These are functions:
		\begin{itemize}
			\item $f=\{(1,a),(2,b)\}$
			\item $f=\{(1,a),(2,a)\}$
		\end{itemize}
		This isn't:
		\begin{itemize}
			\item $f=\{(1,a),(1,b)\}$
		\end{itemize}
	\end{example}
\end{multicols}

\begin{theorem}{Equality of Functions}
	Two functions $f$ and $g$ are equal if:
	\begin{itemize}
		\item They share the same domains / co-domains
		\item They assign the same element from the domain to the same element
	\end{itemize}
	Let $f:A\to B,g:C\to D$:
	\begin{itemize}
		\item $A\neq C\lor B\neq D\implies f\neq g$
		\item $A=C\lor B=D\implies f=g$
	\end{itemize}
\end{theorem}
\begin{multicols}{2}
	{
		\begin{definition}{One-to-One Functions (Injective)}\label{def:one-to-one-functions}
			A function $f:A\to B$ where all values $A$ must correspond to \textit{one and only one} element in $B$: \[\forall a\in A,\forall b\in B.\big(f(a)\neq f(b)\big)\]
		\end{definition}

		\begin{definition}{Bijection}\label{def:bijection}
			A function that is \textit{both} one-to-one \textit{and} onto
		\end{definition}
	}
	\begin{definition}{Onto Functions (Subjective)}\label{def:onto-functions}
		A function $f:A\to B$ where all values $B$ must correspond to \textit{at least an} element in $A$: \[\forall b\in B,\exists a\in A.\big(f(a)=b\big)\]
	\end{definition}
	\begin{definition}{Inverse of Function}\label{def:inverse-function}
		\[f^{-1}(x)=y\iff f(y)=x\]
	\end{definition}
\end{multicols}

\begin{definition}{Compisite Functions}\label{def:composite-function}
	\[\text{domain}(f)=\text{range}(g)\implies f\circ g(x)=f(g(x))\]
	If the composite of the function exists, then:
	\[(f\circ g)^{-1}=g^{-1}\circ f^{-1}\]
\end{definition}

\begin{multicols}{2}
	\begin{definition}{Floor ($\lfloor x\rfloor$)}\label{def:floor-function}
		The biggest integer $n\leq x$
	\end{definition}
	\begin{definition}{Ceiling ($\lceil x\rceil$)}\label{def:floor-function}
		The smallest integer $n\geq x$
	\end{definition}
\end{multicols}
\section{Algorithms}
\begin{multicols}{2}
	\begin{definition}{Algorithm}\label{def:algorithm}
		A sequence of \textit{precise} steps used to solve computational problems
	\end{definition}
	\begin{note}{Input-Output}\label{note:input-output}
		For every input instance, a correct output \textit{must} be produced
	\end{note}
\end{multicols}

\begin{algorithm}
	\caption{Binary Search Algorithm}\label{alg:binary-search}

	\KwIn{$A\gets\{A_1, A_2, \ldots, A_n\}$ where $A_i\in\mathbb{Z}$, $k\in\mathbb{Z}$}
	\KwOut{$i$ where $A_i=k$, or $i=0\implies k\notin A$}

	left$\gets 1$\;
	right$\gets n$\;
	\While{$left<right$}
	{
		$i\gets\lfloor(\text{left}+\text{right})\div 2\rfloor$\;
		\uIf{$A_i=k$}
		{
			\KwRet~$i$\;
		}\uElseIf{$A_i<k$}
		{
			left$\gets i+1$\;
		}\Else{
			right$\gets i$\;
		}
	}
	\KwRet~$0$\;
\end{algorithm}

\begin{algorithm}
	\caption{Insertion Sort}\label{alg:insertion-sort}
	\SetKwFunction{FSwap}{swap}
	\SetKwFunction{FSort}{sort}
	\KwIn{$A\gets\{A_1, A_2, \ldots, A_n\}$ where $n\geq2$}
	\KwOut{$A\gets\{A_1, A_2, \ldots, A_n\}$ where $n\geq2\land A_i\leq A_{i+1}$}

	\For{$\text{i}\gets2$ \KwTo$n$}
	{
		key$\gets A_{\text{i}}$\;
		index$\gets\text{i}-1$\;

		\While{$\text{index}\geq1\land A_{\text{index}}>key$}
		{
			$A_{\text{index}+1}\gets A_{\text{index}}$\;
			$\text{index}\gets\text{index}-1$\;
		}
		$A_{\text{index}+1}\gets\text{key}$\;
	}

\end{algorithm}


\newpage
\subsection{Growth of Functions}
This can be used to determine the growth of functions, and is also mainly
used in the field of \textit{computer science} to analyze algorithms.

\begin{multicols}{2}
	\begin{note}{Proving Big-O}\label{note:proving-big-o}
		To prove that $f(x)=O\big(g(x)\big)$, you must prove the existence of a $C$ and $k$ that fulfill the definition:\[\exists C,k.\big(\forall x>k.(|f(x)|\leq C\times |g(x)|)\big)\]
	\end{note}
	\begin{definition}{Big-O Notation}\label{def:big-o-notation}
		Let $f$ and $g$ be functions. $f(x)$ is $O\big(g(x)\big)$ (read ``$f(x)$ is Big-O of $g(x)$'') when there are constants $C$ and $k$ (the witnesses) such that:\[|f(x)|\leq C|g(x)|,x>k\] This is called the worst-case runtime of an algorithm
	\end{definition}
\end{multicols}

\begin{example}{Identify the Witnesses}\label{ex:find-witnesses}
	Find $C,k$ such that $f(x)=4x^2+2x+1$ is $O(x^2)$
	\begin{align*}
		g(x) & = n^2+n^2+n^2 \\
		     & = 3n^2
	\end{align*}
	$f(x)<g(x) \text{ when } x>1$
	\centering $\displaystyle\therefore C=3,k=1$
\end{example}

\begin{multicols}{2}
	\begin{definition}{Big-$\Omega$}\label{def:big-omega}
		Let $f$ and $g$ be functions. $f(x)$ is $\Omega\big(g(x)\big)$ when there are
		constants $C$ and $k$ such that:\[|f(x)|\geq C|g(x)|\] This is called the
		best-case runtime of an algorithm
	\end{definition}
	\begin{definition}{Big-$\theta$}\label{def:big-theta}
		Let $f$ and $g$ be functions. $f(x)$ is $\theta\big(g(x)\big)$ when:\[f(x)=O\big(g(x)\big)\land f(x)=\Omega\big(g(x)\big)\]
		This is called the average-case runtime of an algorithm
	\end{definition}
\end{multicols}

\newpage
\section{Number Theory}
\begin{definition}{Division}\label{def:division}
	Let $a,b\in\mathbb{Z}$. $a$ divides $b$ ($a|b$) if there exists integer $c$ such that $a\times c=b$
	\[a|b,a,b\in\mathbb{Z}\iff\exists c\in\mathbb{Z}.(a\times c=b)\]
\end{definition}

\begin{theorem}{Basic Division Properties}
	Let $a,b,c\in\mathbb{Z},a\neq 0$:
	\begin{itemize}
		\item $\displaystyle (a|b)\land(a|c)\implies a|(b+c)$
		\item $\displaystyle a|b\implies \forall c\in\mathbb{Z}.\big(a|(b\times c)\big)$
		\item $\displaystyle (a|b)\land(b|c)\implies a|c$
	\end{itemize}
\end{theorem}

\begin{theorem}{Consequence of Division}
	\[\forall a,b,c,m,n\in\mathbb{Z},a\neq0.\Big((a|b)\land(a|c)\implies\big(a|(mb+nc)\big)\Big)\]
	Let $a,b,c,m,n$ be integers where $a\neq0$, and suppose $a|b\land a|c$.
	Then, for any integers m and n, $a|mb+nc$.
\end{theorem}

\begin{theorem}{Division Algorithm}
	Let $a\in\mathbb{Z},d\in\mathbb{Z}^+$. Then there are unique integers $q$
	and $r$ where $0\leq r<d$ such that $a=q\times d+r$
	\[\forall a,q,r\in\mathbb{Z},d\in\mathbb{Z}^+,0\leq r<d.(a=q\times d+r)\]
\end{theorem}

\begin{multicols}{2}
	{
		\begin{definition}{Quotient}
			\[q=a\texttt{ div }d\]
		\end{definition}
		\begin{definition}{Congruency ($\equiv$)}
			Let $a,b\in\mathbb{Z},m\in\mathbb{Z}^+$. $a$ is congruent to $b$ \texttt{mod} $m$ if\ldots
			\begin{itemize}
				\item$m|a-b$
				\item$a \texttt{ mod } m\equiv b \texttt{ mod }m$
				\item$k\in\mathbb{Z},a=b+k\times m$
			\end{itemize}
		\end{definition}
	}
	{
		\begin{definition}{Remainder}
			\[r=a\texttt{ mod }d\]
		\end{definition}

		\begin{theorem}{Preservation of Congruencies}
			Let $a,b,c,d\in\mathbb{Z},m\in\mathbb{Z}^+$. If $a\equiv b\texttt{ mod } m\land c\equiv d\texttt{ mod } m$, then
			\begin{itemize}
				\item$a+c\equiv b+d\hspace{1em}(\texttt{mod } m)$
				\item$a\times c\equiv b\times d\hspace{1em}(\texttt{mod } m)$
			\end{itemize}
		\end{theorem}
	}
\end{multicols}

\section{Induction and Recursion}

\begin{definition}{Proof via. Induction}
    To prove that $P(n)$ is true for $n\in\mathbb{Z}^+$, we must complete these
    two steps:
    \begin{itemize}
        \item \textbf{Basis Step:} Verify that $P(1)$ is \texttt{true}
        \item \textbf{Inductive Step:} Show that 
            $P(k)\implies P(k+1),k\in\mathbb{Z}^+$ is \texttt{true}
    \end{itemize}
\end{definition}

\begin{definition}{Recursion}
    A way to express a definition of an element in terms of itself. There's
    two required steps to recursively define a function:
    \begin{itemize}
        \item \textbf{Basis Step:} Specify the value of the function at 0
        \item \textbf{Recursive Step:} Specify a rule for finding its value at
            an integer from its smaller values at smaller integers
    \end{itemize}
\end{definition}

\section{Relations}
\begin{definition}{Relation}
	Given sets $A,B$, it's a subset of $A\times B$
\end{definition}

\begin{example}{}
	\begin{align*}
		R_1 & = \{(a,b)|a,b\in\mathbb{Z}\land a\leq b\}\subseteq\mathbb{Z}\times\mathbb{Z}        \\
		R_2 & = \{(a,b)|a,b\in\mathbb{Z}\land a<b\}\subseteq\mathbb{Z}\times\mathbb{Z}            \\
		R_3 & = \{(a,b)|a,b\in\mathbb{Z}\land a=b\}\subseteq\mathbb{Z}\times\mathbb{Z}            \\
		R_4 & = \{(a,b)|a,b\in\mathbb{Z}\land a=b+\mathbb{Z}\}\subseteq\mathbb{Z}\times\mathbb{Z} \\
		R_5 & = \{(a,b)|a,b\in\mathbb{Z}\land a|b\}\subseteq\mathbb{Z}\times\mathbb{Z}
	\end{align*}
\end{example}

\begin{multicols}{2}
	{
		\begin{definition}{Reflexivity}
			A relation $R$ on a set $A$ is \textit{reflexive} if and only if:
			\[\forall x.\big(x\in A\implies(x,x)\in R\big)\]
		\end{definition}
	}
	{
		\begin{example}{}
			\begin{align*}
				A & = \{1,2,3\}                                      \\
				R & = \{(1,1),(2,2),(1,3),(3,3)\}                    \\
				R & = \{(3,3),(1,3),(1,1)\}\gets\text{not reflexive}
			\end{align*}
		\end{example}

	}
\end{multicols}
\begin{definition}{Symmetry}
	Relation $R$ on a set $A$ is symmetric if and only if
	\[\forall x\forall y.\big((x,y)\in R\implies(y,x)\in R\big)\]
\end{definition}

\begin{definition}{Anti-Symmetry}
	Relation $R$ on a set $A$ is antisymmetric if and only if
	\[\forall x\forall y.\big((x,y)\in R\land(y,x)\in R\implies(y,x)\in x=y)\]
\end{definition}
\begin{example}{}
	\centering
	\begin{tabular}{cl}
		\multirow{2}{*}{$\leq$}                                                                      & Not symmetric: $3\leq5,5\not\leq3$                   \\
		                                                                                             & Antisymmetric: $a\leq b,b\leq a\implies a=b$         \\
		\hdashline
		\multirow{2}{*}{$>$}                                                                         & Not symmetric: $5>3,3\not>5$                         \\
		                                                                                             & Antisymmetric: $a>b,b>a\implies a=b$                 \\
		\hdashline
		\multirow{2}{*}{$=$}                                                                         & Symmetric                                            \\
		                                                                                             & Antisymmetric: $a=b,b=a\implies a=b$                 \\
		\hdashline
		\multirow{2}{*}{$R=\{(a,b)|a,b\in\mathbb{Z}\land a=-b\}\subseteq\mathbb{Z}\times\mathbb{Z}$} & Symmetric: $(a,-a)\in R\implies (-a,a)\in R$         \\
		                                                                                             & Not antisymmetric: $(a,-a)\land(-a,a)\in R,a\neq -a$ \\
		\hdashline
		\multirow{2}{*}{Let $A=\{1,2,3\}$}                                                           & Not symmetric: $(1,3)\in R,(3,1)\notin R$            \\
		$R=\{(2,3),(3,2),(1,3)\}$                                                                    & Not antisymmetric: $(2,3),(3,2)\in R,2\neq 3$        \\
		\hdashline
	\end{tabular}
\end{example}

\begin{definition}{Transitive}
	A relation $R$ on set $A$ such that
	\[\forall x\forall y\forall z.\big((x,y)\in R\land(y,z)\in R\implies(x,z)\in R\big)\]
\end{definition}

\begin{example}{}
	\begin{align*}
		A & = \{a,b,c\}                         \\
		R & = \{(a,b),(a,a),(b,b),(b,c),(c,b)\} \\
	\end{align*}
	It's nothing, nada, it's\ldots disappointing
\end{example}

\begin{note}{Equivalence Relation}
	A relation that is reflexive, symmetric, and transitive
\end{note}

\newpage
\section{Graphs}
\marginnote{What's a graph without its nodes?}
\begin{definition}{Graph}
	Denoted by $G=(V,E)$, consists of a non-empty set of \textit vertices (or nodes) $V$ and a set of edges $E$
\end{definition}
\begin{multicols}{2}
	\begin{definition}{Adjacent Verticies (Undirected)}
		When the endpoints of an edge $e$ are vertices $a$ and $b$, the verticies
		are considered to be \textit{adjacent} (or \textit{neighbors}) with one
		another.
		\bl
		That edge is called an \textit{incident} edge, \textit{connecting} verticies
		$a$ and $b$
	\end{definition}
	\begin{definition}{Adjacent Verticies (Directed)}
		When $(a,b)$ is an edge of a directed graph $G$, $a$ is \textit{adjacent to}
		$b$, and $a$ is \textit{adjacent from} $b$.
		\bl
		Vertex $a$ is called the \textit{initial vertex}, and $b$ is called
		the \textit{terminal} or \textit{end vertex} of $(u,v)$
	\end{definition}
\end{multicols}

\begin{definition}{Neighborhood $\big(N(v)\big)$}
	``The set of all neighbors of $u$'' of a graph $G=(V,E)$, denoted by ($N(v)$)
	\bl
	If $A$ is a subset of $V$, $N(A)$ is the set of verticies in $G$ that are
	adjacent to at least one vertex in $A$: \[V=\bigcup_{v\in A}N(v)\]
\end{definition}

\begin{multicols}{2}
	\begin{definition}{Degree (Undirected Graph) \big(\texttt{deg}($v$)\big)}
		The number of edges incident with it. A loop contributes \textit{twice} to
		the degree of that vertex
	\end{definition}
	\begin{definition}{Degree (Directed Graph) \big(\texttt{deg}$^{\pm}$($v$)\big)}
		The number of edges incident with it. A loop contributes \textit{twice} to
		the degree of that vertex
	\end{definition}
\end{multicols}

\begin{definition}{Infinite Graphs}
	If $|V|=\infty$, then the graph is referred to as an \textit{infinite} graph,
	otherwise it's called a \textit{finite} graph
\end{definition}


\begin{example}{Neighborhoods and Degrees}
	\centering
	\captionof{figure}{Neighborhoods Example}\label{fig:neighborhoods}
	\begin{graph}
		\node(1) {\emoji{apple}};
		\node[right of=1] (2) {\emoji{banana}};
		\node[below of=1] (3) {\emoji{mango}};
		\node[right of=2] (4) {\emoji{orange}};
		\node[right of=3] (5) {\emoji{coconut}};

		\draw(1) to [bend right] (2);
		\draw(1) to (2);
		\draw(2) to [bend right] (1);
		\draw(1) to (3);
		\draw(1) to (5);
		\draw(2) to (3);
		\draw(2) to (5);
		\draw(2) to (4);
		\draw(4) to (5);
		\draw(4) to [in=270,out=0,looseness=4] (4);
	\end{graph}
	\bl
	\captionof{table}{Table of Neighbors and Degrees}
	\begin{tabular}{ccc}
		\multicolumn{1}{c}{\textbf{Vertex}} &
		\multicolumn{1}{c}{\textbf{Degree}} &
		\multicolumn{1}{c}{\textbf{Neighborhood}}                      \\
		\midrule
		\emoji{mango}                       &
		2                                   &
		\{\emoji{apple},\emoji{banana}\}                               \\
		\emoji{coconut}                     &
		3                                   &
		\{\emoji{apple},\emoji{banana},\emoji{orange}\}                \\
		\emoji{orange}                      &
		4                                   &
		\{\emoji{orange},\emoji{banana},\emoji{coconut}\}              \\
		\emoji{apple}                       &
		5                                   &
		\{\emoji{mango},\emoji{banana},\emoji{coconut}\}               \\
		\emoji{banana}                      &
		6                                   &
		\{\emoji{apple},\emoji{mango},\emoji{coconut},\emoji{orange}\} \\
	\end{tabular}
\end{example}

\begin{note}{Sum of Degrees}
	When adding the degrees of all verticies in graph $G=(V,E)$, you'll find
	that each edge contributes \textit{two} to the sum of degrees, since
	each edge is incident with exactly two verticies
\end{note}

\begin{theorem}{Handshake Theorem}
	If $G=(v,E)$ is an undirected graph with $|E|=m$ edges, then
	\[\sum_{v\in V}\texttt{deg($v$)}=\sum_{v\in V_1}\texttt{deg($v$)}+\sum_{v\in V_2}\texttt{deg($v$)}=2\times m\]
	This applies even if multiple edges and loops are present
\end{theorem}

\begin{example}{Handshake}
	We can see this theorem in effect if we look back at
	\hyperref[fig:neighborhoods]{Figure 1}:
	\begin{align*}
		2\times m = & \sum_{v\in V}\texttt{deg($v$)} \\
		=           & 2 + 3 + 4 + 5 + 6              \\
		2\times m = & 20                             \\
		m =         & 10
	\end{align*}
\end{example}

\newpage
\begin{multicols}{2}
	\begin{theorem}{Consequences of Handshaking}
		In an undirected graph, the  sum of degree of nodes with odd degrees is
		\textit{even}.
	\end{theorem}
	\begin{theorem}{Directed Handshake}
		Let $G=(V,E)$ be a directed graph:
		\[\sum_{v\in V}\texttt{deg}^-(v)=\sum_{v\in V}\texttt{deg}^+(v)=|E|\]
	\end{theorem}
\end{multicols}

\begin{table}[h!]
	\centering
	\caption{Graph Terminology}
	\begin{tabular}{llll}
		\multicolumn{1}{c}{\textbf{Type}}      &
		\multicolumn{1}{c}{\textbf{Direction}} &
		\multicolumn{1}{c}{\textbf{Edges}}     &
		\multicolumn{1}{c}{\textbf{Loops}}                                   \\
		\midrule
		Simple Graph                           & Undirected & Singular & No  \\
		Multigraph                             & Undirected & Multiple & No  \\
		Pseudograph                            & Undirected & Multiple & Yes \\
		Simple Directed Graph                  & Directed   & Singular & No  \\
		Directed Multigraph                    & Directed   & Multiple & Yes \\
		Mixed Graph                            & Both       & Multiple & Yes \\
	\end{tabular}
\end{table}

\begin{multicols}{2}
	\begin{minipage}{\linewidth}
		\centering
		\captionof{figure}{Simple Graph}
		\begin{graph}
			\node (1) {\emoji{apple}};
			\node (2) [below of=1] {\emoji{banana}};
			\node (3) [right of=1]{\emoji{cat}};
			\node (4) at (0.85,-0.85) {\emoji{dog}};
			\node (5) [below of=3] {\emoji{elephant}};

			\draw (1) -- (3);
			\draw (3) -- (4);
			\draw (4) -- (2);
			\draw (2) -- (5);
		\end{graph}
	\end{minipage}
	\begin{minipage}{\linewidth}
		\centering
		\captionof{figure}{Multigraph}
		\begin{graph}
			\node (1) {\emoji{apple}};
			\node (2) [below of=1] {\emoji{banana}};
			\node (3) [right of=1]{\emoji{cat}};
			\node (4) at (0.85,-0.85) {\emoji{dog}};
			\node (5) [below of=3] {\emoji{elephant}};

			\draw (1) -- (3);
			\draw (1) -- (4);
			\draw (2) -- (4);
			\draw (4) -- (5);
		\end{graph}
	\end{minipage}
	\begin{minipage}{\linewidth}
		\centering
		\captionof{figure}{Pseudograph}
		\begin{graph}
			\node (1) {\emoji{apple}};
			\node (2) [below of=1] {\emoji{banana}};
			\node (3) [right of=1]{\emoji{cat}};
			\node (4) at (0.85,-0.85) {\emoji{dog}};
			\node (5) [below of=3] {\emoji{elephant}};

			\draw (1) -- (3);
			\draw (1) -- (4);
			\draw (2) -- (4);
			\draw (4) -- (5);
			\draw (5) to [out=270,in=330,looseness=5] (5);
		\end{graph}
	\end{minipage}
	\begin{minipage}{\linewidth}
		\centering
		\captionof{figure}{Simple Directed Graph}
		\begin{graph}
			\node (1) {\emoji{apple}};
			\node (2) [below of=1] {\emoji{banana}};
			\node (3) [right of=1]{\emoji{cat}};
			\node (4) at (0.85,-0.85) {\emoji{dog}};
			\node (5) [below of=3] {\emoji{elephant}};

			\draw[<-] (1) -- (3);
			\draw[->] (1) -- (4);
			\draw[<-] (2) -- (4);
			\draw[->] (2) -- (5);
		\end{graph}
	\end{minipage}
	\begin{minipage}{\linewidth}
		\centering
		\captionof{figure}{Directed Multigraph}
		\begin{graph}
			\node (1) {\emoji{apple}};
			\node (2) [below of=1] {\emoji{banana}};
			\node (3) [right of=1]{\emoji{cat}};
			\node (4) at (0.85,-0.85) {\emoji{dog}};
			\node (5) [below of=3] {\emoji{elephant}};

			\draw[<->] (1) -- (3);
			\draw[->] (1) -- (4);
			\draw[->] (2) -- (4);
			\draw[->] (4) -- (5);
		\end{graph}
	\end{minipage}
	\begin{minipage}{\linewidth}
		\centering
		\captionof{figure}{Mixed Graph}
		\begin{graph}
			\node (1) {\emoji{apple}};
			\node (2) [below of=1] {\emoji{banana}};
			\node (3) [right of=1]{\emoji{cat}};
			\node (4) at (0.85,-0.85) {\emoji{dog}};
			\node (5) [below of=3] {\emoji{elephant}};

			\draw (1) -- (3);
			\draw[->] (1) -- (4);
			\draw (2) -- (4);
			\draw[->] (4) -- (5);
			\draw[<-] (5) to [out=270,in=330,looseness=5] (5);
		\end{graph}
	\end{minipage}
\end{multicols}
\end{document}
